run.sh
@@ -1,5 +1,7 @@
 #!/bin/bash 
-fstar.exe --record_hints --use_hints --odir fstar_out --codegen OCaml BDD2.fst AVL.fst BinTree.fst BDD.fst MapAVL.fst SetAVL.fst Compare.fst --query_stats 
+
+# AVL.fst BinTree.fst BDD.fst MapAVL.fst SetAVL.fst Compare.fst
+fstar.exe --record_hints --use_hints --odir fstar_out --codegen OCaml BDD2.fst # --query_stats 
 cd fstar_out 
-ocamlbuild BDD2.native -package fstarlib,batteries
+# ocamlbuild BDD2.native -package fstarlib,batteries
 cd ..
